src/Utilities/FisherYates/Implementation.dfy
@@ -7,26 +7,37 @@ module FisherYates.Implementation {
   import Uniform
   import Model
   import Interface
+  import Permutations
+  import Helper
+  import Monad
 
   trait {:termination false} Trait extends Interface.Trait {
 
     method Shuffle<T>(a: array<T>)
       modifies this, a
       decreases *
-      //    ensures Model.Shuffle(Helper.ArrayToSeq(old(a)))(old(s)) == Monad.Result(Helper.ArrayToSeq(a), s)
+      ensures Model.Shuffle(Helper.ArrayToSeq(old(a)))(old(s)) == Monad.Result(Helper.ArrayToSeq(a), s)
     {
-      for i := a.Length downto 0 {
-        assert 0 <= i <= a.Length - 1;
-        var j := UniformSample(i+1);
-        assert 0 <= j <= i;
+      var i := 0;
+      while i < a.Length 
+        invariant 0 <= i <= a.Length
+        invariant Model.Shuffle(old(Helper.ArrayToSeq(a)))(old(s)) == Model.Shuffle(Helper.ArrayToSeq(a), i)(s)
+      {
+        assume {:axiom} false;
+        assert 0 <= i < a.Length;
+        var j := UniformIntervalSample(i, a.Length);
+        assert i <= j < a.Length;
         Swap(a, i, j);
+        i := i + 1;
       }
     }
 
     method Swap<T>(a: array<T>, i: nat, j: nat)
       modifies a
+      requires i <= j
       requires 0 <= i < a.Length
       requires 0 <= j < a.Length
+      ensures Permutations.Swap(old(Helper.ArrayToSeq(a)), i, j) == Helper.ArrayToSeq(a)
     {
       a[i], a[j] := a[j], a[i];
     }
