src/Utilities/FisherYates/Model.dfy
@@ -7,11 +7,57 @@ module FisherYates.Model {
   import Monad
   import Rand
   import Permutations
+  import Uniform
+  import Loops
 
-  // TODO: add correct version
-  function Shuffle<T>(xs: seq<T>): (f: Monad.Hurd<seq<T>>) {
-    (s: Rand.Bitstream) =>
-      Monad.Result(xs, s)
+  ghost function Shuffle<T>(xs: seq<T>, i: nat := 0): (f: Monad.Hurd<seq<T>>) 
+    requires 0 <= i <= |xs|
+  {
+    assume {:axiom} false; // assume termination
+    if i == |xs| then
+      Monad.Return(xs)
+    else 
+      Monad.Bind(
+        Uniform.Model.IntervalSample(i, |xs|),
+        (j: nat) requires i <= j < |xs| => 
+          var ys := Permutations.Swap(xs, i, j);
+          Shuffle(ys, i + 1)
+      )
   }
+  // TODO: add correct version
+/*   function Shuffle<T>(xs: seq<T>): (f: Monad.Hurd<seq<T>>) {
+    Monad.Map(
+      Loops.While(ShuffleWhileLoopCondition, ShuffleWhileLoopBody)((xs, 0)), 
+      (x: (seq<T>, nat)) => x.0
+    )
+  }
+
+  function ShuffleWhileLoopCondition<T>(x: (seq<T>, nat)): bool {
+    x.1 < |x.0|
+  }
+
+  function ShuffleWhileLoopBody<T>(x: (seq<T>, nat)): Monad.Hurd<(seq<T>, nat)> {
+    Monad.Bind(
+      Uniform.Model.IntervalSample(x.1, |x.0|),
+      (j: nat) => 
+        var ys := Permutations.Swap(x.0, 0, j); 
+        Monad.Return((ys, x.1 + 1))
+    )
+  } */
+
+/*   ghost function ShuffleTailRecursive<T>(xs: seq<T>): Monad.Hurd<seq<T>> 
+    decreases |xs|
+  {
+    if |xs| == 0 then 
+      Monad.Return(xs)
+    else 
+      Monad.Bind(
+        Uniform.Model.Sample(|xs|),
+        (j: nat) requires 0 <= j < |xs| => 
+          var ys := Permutations.Swap(xs, 0, j);          
+          Monad.Map(ShuffleTailRecursive(ys[1..]), (zs: seq<T>) => [ys[0]] + zs)
+          // ShuffleTailRecursiveCurried(ShuffleTailRecursiveCurried(Permutations.Substitute(xs[1..], j-1, xs[0])).Map((zs: set<T>) => [xs[j]] + zs))
+      )
+  } */
 
 }
